devel/Iron/SystemF2Effect/Store/Wf.v
@@ -63,19 +63,46 @@ Qed.
 Hint Resolve wfFS_sregion_cons.
 
 
+Lemma deallocate_typeb
+ :  forall ke te se sp p b t
+ ,  TYPEB  ke te se sp b t
+ -> TYPEB  ke te se sp (deallocate p b) t.
+Proof.
+ intros.
+ destruct b.
+ - snorm. subst.
+   inverts H. eauto.
+ - snorm.
+Qed.
+
+
+Lemma deallocate_storet
+ :  forall se sp ss p
+ ,  STORET se sp ss
+ -> STORET se sp (map (deallocate p) ss).
+Proof.
+ intros.
+ unfold STORET in *.
+ eapply Forall2_map_left.
+ eapply Forall2_impl.
+  intros.
+  eapply deallocate_typeb. eauto. auto.
+Qed.
+
+
 (* Deallocating a region preserves well-formedness of the store. *)
 Lemma wfFS_stack_pop
  :  forall se sp ss fs p
- ,  WfFS se sp ss               (fs :> FUse p)
- -> WfFS se sp (deallocate p ss) fs.
+ ,  WfFS se sp ss                     (fs :> FUse p)
+ -> WfFS se sp (map (deallocate p) ss) fs.
 Proof.
  intros.
- unfold WfFS in *. 
- admit. (* wfFS after region dealloc *)
-(*
- rip. 
- unfold STOREP in *.
-  eauto.
-*)
-Qed.
+ unfold WfFS in *. rip.
+ - unfold STOREM in *.
+   rewrite map_length. auto.
 
+ - eapply deallocate_storet. auto.
+ 
+ - unfold STOREP in *.
+   snorm.
+Qed.
